\begin{prooftree}
\AxiomC{[$B \rightarrow B^*$]}
\RightLabel{[$\neg$L]}
\UnaryInfC{$\neg B^*, B \rightarrow $}
\RightLabel{[$\land$L]}
\UnaryInfC{$(\neg B^* \land \neg C^*), B \rightarrow $}
\RightLabel{[$\neg$R]}
\UnaryInfC{$B \rightarrow \neg (\neg B^* \land \neg C^*)$}
\AxiomC{[$C \rightarrow C^*$]}
\RightLabel{[$\neg$L]}
\UnaryInfC{$\neg C^*, C \rightarrow $}
\RightLabel{[$\land$L]}
\UnaryInfC{$(\neg B^* \land \neg C^*), C \rightarrow $}
\RightLabel{[$\neg$R]}
\UnaryInfC{$C \rightarrow \neg (\neg B^* \land \neg C^*)$}
\RightLabel{[$\lor$L]}
\BinaryInfC{$(B \lor C) \rightarrow \neg (\neg B^* \land \neg C^*)$}
\RightLabel{[$\supset$R]}
\UnaryInfC{$ \rightarrow ((B \lor C) \supset \neg (\neg B^* \land \neg C^*))$}
\AxiomC{[$B^* \rightarrow B$]}
\RightLabel{[$\lor$R]}
\UnaryInfC{$B^* \rightarrow (B \lor C)$}
\RightLabel{[$\neg$R]}
\UnaryInfC{$ \rightarrow (B \lor C), \neg B^*$}
\AxiomC{[$C^* \rightarrow C$]}
\RightLabel{[$\lor$R]}
\UnaryInfC{$C^* \rightarrow (B \lor C)$}
\RightLabel{[$\neg$R]}
\UnaryInfC{$ \rightarrow (B \lor C), \neg C^*$}
\RightLabel{[$\land$R]}
\BinaryInfC{$ \rightarrow (B \lor C), (\neg B^* \land \neg C^*)$}
\RightLabel{[$\neg$L]}
\UnaryInfC{$\neg (\neg B^* \land \neg C^*) \rightarrow (B \lor C)$}
\RightLabel{[$\supset$R]}
\UnaryInfC{$ \rightarrow (\neg (\neg B^* \land \neg C^*) \supset (B \lor C))$}
\RightLabel{[$\land$R]}
\BinaryInfC{$ \rightarrow ((B \lor C) \equiv \neg (\neg B^* \land \neg C^*))$}
\end{prooftree}
