\begin{prooftree}
\AxiomC{[$B^* \rightarrow B$]}
\AxiomC{[$C \rightarrow C^*$]}
\RightLabel{[$\supset$L]}
\BinaryInfC{$(B \supset C), B^* \rightarrow C^*$}
\RightLabel{[XL]}
\UnaryInfC{$B^*, (B \supset C) \rightarrow C^*$}
\RightLabel{[$\supset$R]}
\UnaryInfC{$(B \supset C) \rightarrow (B^* \supset C^*)$}
\RightLabel{[$\supset$R]}
\UnaryInfC{$ \rightarrow ((B \supset C) \supset (B^* \supset C^*))$}
\AxiomC{[$B \rightarrow B^*$]}
\AxiomC{[$C^* \rightarrow C$]}
\RightLabel{[$\supset$L]}
\BinaryInfC{$(B^* \supset C^*), B \rightarrow C$}
\RightLabel{[XL]}
\UnaryInfC{$B, (B^* \supset C^*) \rightarrow C$}
\RightLabel{[$\supset$R]}
\UnaryInfC{$(B^* \supset C^*) \rightarrow (B \supset C)$}
\RightLabel{[$\supset$R]}
\UnaryInfC{$ \rightarrow ((B^* \supset C^*) \supset (B \supset C))$}
\RightLabel{[$\land$R]}
\BinaryInfC{$ \rightarrow ((B \supset C) \equiv (B^* \supset C^*))$}
\end{prooftree}
