\begin{prooftree}
\AxiomC{$(\neg B^* \land \neg C^*) \rightarrow (\neg B^* \land \neg C^*)$}
\RightLabel{[$\neg$L]}
\UnaryInfC{$\neg (\neg B^* \land \neg C^*), (\neg B^* \land \neg C^*) \rightarrow $}
\RightLabel{[$\neg$R]}
\UnaryInfC{$(\neg B^* \land \neg C^*) \rightarrow \neg \neg (\neg B^* \land \neg C^*)$}
\RightLabel{[$\neg$L]}
\UnaryInfC{$\neg \neg \neg (\neg B^* \land \neg C^*), (\neg B^* \land \neg C^*) \rightarrow $}
\RightLabel{[XL]}
\UnaryInfC{$(\neg B^* \land \neg C^*), \neg \neg \neg (\neg B^* \land \neg C^*) \rightarrow $}
\RightLabel{[$\neg$R]}
\UnaryInfC{$\neg \neg \neg (\neg B^* \land \neg C^*) \rightarrow \neg (\neg B^* \land \neg C^*)$}
\end{prooftree}
